examples/low-level/crypto/Crypto.AEAD.PRF_MAC.fst
@@ -12,6 +12,7 @@ open Crypto.Plain
 open Crypto.Symmetric.Bytes
 
 open Crypto.AEAD.Invariant
+open Crypto.AEAD.Encrypt.Invariant
 
 module HS  = FStar.HyperStack
 
@@ -77,6 +78,9 @@ let prf_mac_ensures (i:id) (t:PRF.state i) (k_0: CMA.akey t.mac_rgn i) (x:PRF.do
 
 (*****)
 
+(*
+ * AEAD entries remain same after prf mac, separating it makes things go a bit faster
+ *)
 private val lemma_aead_entries_are_same_after_prf_mac
   (#i:id)
   (#rw:rw)
@@ -85,15 +89,16 @@ private val lemma_aead_entries_are_same_after_prf_mac
   (x:PRF.domain_mac i)
   (h0 h1:mem)
   (mac:CMA.state (i, x.iv)) : Lemma
-  (requires (h0 `HS.contains` (st_ilog aead_st) /\
-             prf_mac_ensures i aead_st.prf k_0 x h0 mac h1))
+  (requires (h0 `HS.contains` (st_ilog aead_st) /\            //initial heap contains the aead log
+             prf_mac_ensures i aead_st.prf k_0 x h0 mac h1))   //h0 and h1 are related by prf_mac_ensures
   (ensures  (let entries_0 = HS.sel #(aead_entries i) h0 aead_st.log in
              let entries_1 = HS.sel #(aead_entries i) h1 aead_st.log in
-	     entries_0 == entries_1))
-#set-options "--z3rlimit 100"
+	     entries_0 == entries_1))  //aead entries are same in h0 and h1
 let lemma_aead_entries_are_same_after_prf_mac #i #rw aead_st k_0 x h0 h1 mac = ()
 
-#reset-options
+(*
+ * Freshness of nonces is preserved by prf_mac, follows the from preservation of aead entries by prf_mac
+ *)
 private val frame_fresh_nonce_st_prf_mac
   (#i:id)
   (#rw:rw)
@@ -162,7 +167,11 @@ let frame_refines_aead_entries_prf_mac #i #rw aead_st k_0 x h0 h1 mac =
     frame_refines_entries_h i aead_st.prf.mac_rgn table_0 aead_ent_0 h0 h1;
     frame_refines_entries_prf_append table_0 aead_ent_0 h1 (Seq.create 1 (PRF.Entry x mac))
 
-private val lemma_iv_of_x_is_unused_prf_mac
+(*
+ * unused_aead_iv_for_prf for x.iv is preserved by prf_mac
+ * since prf_mac does not add any otp entries, and leaves an unset mac entry for x.iv after completion
+ *)
+private val frame_unused_aead_iv_for_prf_x_prf_mac
   (#i:id)
   (#rw:rw)
   (aead_st:aead_state i rw{safeMac i})
@@ -175,24 +184,13 @@ private val lemma_iv_of_x_is_unused_prf_mac
              prf_mac_ensures i aead_st.prf k_0 x h0 mac h1))
   (ensures  (let table_1 = HS.sel h1 (itable i aead_st.prf) in
              unused_aead_iv_for_prf table_1 x.iv h1))
-let lemma_iv_of_x_is_unused_prf_mac #i #rw aead_st k_0 x mac h0 h1 = ()
+let frame_unused_aead_iv_for_prf_x_prf_mac #i #rw aead_st k_0 x mac h0 h1 = ()
 
 (*
- * Factoring it out, makes the proof go faster
+ * unused_aead_iv_for_prf for any iv <> x.iv is preserved by prf_mac
+ * since prf_mac does not add any entries in the prf table for iv <> x.iv, and does not modify existing references in the mac_rgn
  *)
-val frame_cma_mac_is_unset_h
-  (i:CMA.id)
-  (r:rid{is_eternal_region r})
-  (r':rid{r' `HS.is_above` r})
-  (mac_st:CMA.state i)
-  (h0 h1:mem) : Lemma
-  (requires (CMA.mac_is_unset i r mac_st h0 /\
-             HS.modifies_transitively (Set.singleton r') h0 h1 /\
-             HS.modifies_ref r TSet.empty h0 h1))
-  (ensures  (CMA.mac_is_unset i r mac_st h1))
-let frame_cma_mac_is_unset_h i r r' mac_st h0 h1 = ()
-
-private val frame_unused_aead_iv_different_from_x_prf_mac
+private val frame_unused_aead_iv_for_prf_different_from_x_prf_mac
   (#i:id)
   (#rw:rw)
   (aead_st:aead_state i rw{safeMac i})
@@ -204,10 +202,10 @@ private val frame_unused_aead_iv_different_from_x_prf_mac
   (requires (let table_0 = HS.sel h0 (itable i aead_st.prf) in
              unused_aead_iv_for_prf table_0 iv h0 /\
              prf_mac_ensures i aead_st.prf k_0 x h0 mac h1 /\
-	     not (iv = x.iv)))
+	     iv <> x.iv))
   (ensures  (let table_1 = HS.sel h1 (itable i aead_st.prf) in
              unused_aead_iv_for_prf table_1 iv h1))
-let frame_unused_aead_iv_different_from_x_prf_mac #i #rw aead_st k_0 x mac h0 h1 iv =
+let frame_unused_aead_iv_for_prf_different_from_x_prf_mac #i #rw aead_st k_0 x mac h0 h1 iv =
   let table_0 = HS.sel h0 (itable i aead_st.prf) in
   let table_1 = HS.sel h1 (itable i aead_st.prf) in
   let dom_0 = {iv=iv; ctr=PRF.ctr_0 i} in
@@ -219,7 +217,11 @@ let frame_unused_aead_iv_different_from_x_prf_mac #i #rw aead_st k_0 x mac h0 h1
      | None   ->
        frame_cma_mac_is_unset_h (i, iv) CMA.(mac_range.region) aead_st.prf.rgn mac_range h0 h1)
 
-private val frame_unused_aead_iv_prf_mac
+(*
+ * for all fresh nonces, unused_aead_iv_for_prf holds after prf_mac
+ * case analysis on iv = x.iv or iv <> x.iv
+ *)
+private val frame_unused_aead_iv_for_prf_prf_mac
   (#i:id)
   (#rw:rw)
   (aead_st:aead_state i rw{safeMac i})
@@ -233,10 +235,17 @@ private val frame_unused_aead_iv_prf_mac
 	     prf_mac_ensures i aead_st.prf k_0 x h0 mac h1))
   (ensures  (let table_1 = HS.sel h1 (itable i aead_st.prf) in
 	     unused_aead_iv_for_prf table_1 iv h1))
-let frame_unused_aead_iv_prf_mac #i #rw aead_st k_0 x mac h0 h1 iv =
-  if iv = x.iv then lemma_iv_of_x_is_unused_prf_mac #i #rw aead_st k_0 x mac h0 h1
-  else              frame_unused_aead_iv_different_from_x_prf_mac #i #rw aead_st k_0 x mac h0 h1 iv
+let frame_unused_aead_iv_for_prf_prf_mac #i #rw aead_st k_0 x mac h0 h1 iv =
+  if iv = x.iv then frame_unused_aead_iv_for_prf_x_prf_mac #i #rw aead_st k_0 x mac h0 h1
+  else              frame_unused_aead_iv_for_prf_different_from_x_prf_mac #i #rw aead_st k_0 x mac h0 h1 iv
 
+(*
+ * framing of fresh_nonces_are_unused by prf_mac
+ * the proof follows from:
+     -- a nonce fresh before prf_mac is fresh after prf_mac (frame_fresh_nonce_st_prf_mac)
+     -- if unused_aead_iv_for_prf for a fresh nonce before prf_mac (ensured by inv), then unused_aead_iv_for_prf for that nonce
+        after prf_mac (frame_unused_aead_iv_for_prf_prf_mac)
+ *)
 private val frame_fresh_nonces_are_unused_prf_mac
   (#i:id)
   (#rw:rw)
@@ -253,8 +262,11 @@ private val frame_fresh_nonces_are_unused_prf_mac
 let frame_fresh_nonces_are_unused_prf_mac #i #rw aead_st k_0 x h0 h1 mac =
   let open FStar.Classical in
   forall_intro (move_requires (frame_fresh_nonce_st_prf_mac aead_st k_0 x h0 h1 mac));
-  forall_intro (move_requires (frame_unused_aead_iv_prf_mac aead_st k_0 x mac h0 h1))
+  forall_intro (move_requires (frame_unused_aead_iv_for_prf_prf_mac aead_st k_0 x mac h0 h1))
 
+(*
+ * framing of inv by prf_mac
+ *)
 private val frame_inv_prf_mac
   (#i:id)
   (#rw:rw)
@@ -272,10 +284,10 @@ let frame_inv_prf_mac #i #rw aead_st k_0 x h0 h1 mac =
     frame_fresh_nonces_are_unused_prf_mac aead_st k_0 x h0 h1 mac
   end
 
-val prf_mac_find_unchanged (#i:id) (#rw:rw) (aead_st:aead_state i rw)
-			   (k_0:CMA.akey aead_st.prf.mac_rgn i)
-			   (x:PRF.domain_mac i)
-			   (h0:mem) (h1:mem) (e:PRF.entry aead_st.prf.mac_rgn i)
+private val prf_mac_find_unchanged (#i:id) (#rw:rw) (aead_st:aead_state i rw)
+			           (k_0:CMA.akey aead_st.prf.mac_rgn i)
+			           (x:PRF.domain_mac i)
+			           (h0:mem) (h1:mem) (e:PRF.entry aead_st.prf.mac_rgn i)
    : Lemma (requires (let open PRF in
 		      prf i /\ (
 		      let t0 = HS.sel h0 (itable i aead_st.prf) in
@@ -299,7 +311,7 @@ let prf_mac_find_unchanged #i #rw aead_st k_0 x h0 h1 e =
       Strengthening the spec of PRF.prf_mac to show that 
       it leaves the table unchanged except at one location
  *)      
-val prf_mac_0
+private val prf_mac_0
   (#i:id)
   (#rw:rw)
   (aead_st:aead_state i rw)
@@ -318,12 +330,6 @@ let prf_mac_0 #i #rw aead_st k_0 x =
   end;
   mac
 
-let ak_live (#i:CMA.id) (r:rid) (ak:CMA.state i) (h:mem) = 
-    let open CMA in 
-    ak.region = r /\
-    Buffer.live h ak.s /\
-    MAC.norm h ak.r
-
 (*+ prf_mac_enc:
       A wrapper for PRF.prf_mac, specialized for its use in AEAD.Encrypt.encrypt
 **)      
@@ -338,22 +344,22 @@ val prf_mac_enc
   (x:PRF.domain_mac i)
   : ST (CMA.state (i,x.iv))
        (requires (fun h0 -> 
-		   enc_dec_separation aead_st aad plain cipher_tagged /\
-		   enc_dec_liveness aead_st aad plain cipher_tagged h0 /\
-		   inv aead_st h0 /\
-                   (safeMac i ==> fresh_nonce_st x.iv aead_st h0)))
+		   enc_dec_separation aead_st aad plain cipher_tagged /\    //separation invariants
+		   enc_dec_liveness aead_st aad plain cipher_tagged h0 /\   //liveness invariants hold in h0
+		   inv aead_st h0 /\                                        //main stateful invariant holds in h0
+                   (safeMac i ==> fresh_nonce_st x.iv aead_st h0)))        //x.iv is fresh for aead_st in h0
        (ensures (fun h0 ak h1 -> 
-       		   enc_dec_liveness aead_st aad plain cipher_tagged h1 /\
-		   prf_mac_ensures i aead_st.prf k_0 x h0 ak h1 /\
-		   BufferUtils.prf_mac_modifies aead_st.log_region aead_st.prf.mac_rgn h0 h1 /\
-   		   ak_live PRF.(aead_st.prf.mac_rgn) ak h1 /\
-		   inv aead_st h1 /\
+       		   enc_dec_liveness aead_st aad plain cipher_tagged h1 /\                        //liveness invariants hold in h1
+		   prf_mac_ensures i aead_st.prf k_0 x h0 ak h1 /\                                //h0 and h1 are related by prf_mac_ensures
+		   BufferUtils.prf_mac_modifies aead_st.log_region aead_st.prf.mac_rgn h0 h1 /\  //prf_mac only touches the prf region and children, and does not modify any existing reference in the mac region
+   		   ak_live PRF.(aead_st.prf.mac_rgn) ak h1 /\                                    //ak_live
+		   inv aead_st h1 /\                                                             //prf_mac preserves the main stateful invariant
                    (safeMac i ==>
 		    (let table_1 = HS.sel h1 (itable i aead_st.prf) in
-		     fresh_nonce_st x.iv aead_st h1 /\
-		     is_mac_for_iv aead_st ak h1 /\
-		     unused_mac_exists table_1 x h1 /\
-		     none_above (PRF.incr i x) table_1))))
+		     fresh_nonce_st x.iv aead_st h1 /\                                           //x.iv is still fresh in h1 (no modifications to the aead log)
+		     is_mac_for_iv aead_st ak h1 /\                                              //ak is the mac entry for x.iv in the prf table
+		     unused_mac_exists table_1 x h1 /\                                            //unused mac exists in the prf table
+		     none_above (PRF.incr i x) table_1))))                                       //no otp entries after prf_mac
 let prf_mac_enc #i #rw aead_st #aadlen aad #len plain cipher_tagged k_0 x = 
  let h0 = get () in
  let ak = prf_mac_0 aead_st k_0 x in
@@ -395,561 +401,8 @@ let prf_mac_dec #i #rw aead_st #aadlen aad #len plain cipher_tagged k_0 x =
   ak
 
 #reset-options
-let post_prf_mac
-  (#i:id)
-  (#rw:rw)
-  (aead_st:aead_state i rw)
-  (nonce:Cipher.iv (alg i))
-  (h:mem) =
-  let x = {iv=nonce; ctr=PRF.ctr_0 i} in
-  inv aead_st h                        /\             //invariant holds
-  (safeMac i ==>
-    (let table = HS.sel h (itable i aead_st.prf) in
-     fresh_nonce_st nonce aead_st h    /\             //nonce remains fresh (i.e. it is not in the aead_entries in h)
-     unused_mac_exists table x h /\                   //unused mac exists for the nonce
-     none_above (PRF.incr i x) table))               //no OTP entries exist for the nonce in the PRF table
-
-module Plain = Crypto.Plain
-
-let enc_dec_liveness_and_separation (#i:id) (#rw:rw) (aead_st:aead_state i rw)
-                                    (#aadlen:nat) (aad:lbuffer aadlen)
-				    (#plainlen:nat) (plain: plainBuffer i plainlen)
-				    (#cipherlen:nat) (cipher:lbuffer cipherlen)
-                                    (h:mem)
-  = enc_dec_liveness aead_st aad plain cipher h /\
-    enc_dec_separation aead_st aad plain cipher /\
-    aead_liveness aead_st h
-
-let enxor_pre
-  (#i:id)
-  (#rw:rw)
-  (#aadlen:aadlen_32)
-  (#plainlen:txtlen_32{plainlen <> 0ul /\ safelen i (v plainlen) (otp_offset i)})
-  (aead_st:aead_state i rw)
-  (nonce:Cipher.iv (alg i))
-  (aad:lbuffer (v aadlen))
-  (plain:plainBuffer i (v plainlen))
-  (cipher:lbuffer (v plainlen))
-  (h0:mem) =
-  let dom_0 = {iv=nonce; ctr=PRF.ctr_0 i} in
-  inv aead_st h0                                              /\
-  enc_dec_liveness_and_separation aead_st aad plain cipher h0 /\
-  (safeMac i ==>
-    (let prf = itable i aead_st.prf in
-     let table_0 = HS.sel h0 prf in
-     fresh_nonce_st nonce aead_st h0  /\
-     unused_mac_exists table_0 dom_0 h0))
-
-let ctagbuf (plainlen:txtlen_32) = lbuffer (v plainlen + v MAC.taglen)
-
-let cbuf (#plainlen:txtlen_32) (ct:ctagbuf plainlen) : lbuffer (v plainlen) = 
-  Buffer.sub ct 0ul plainlen
-
-let ctag (#plainlen:txtlen_32) (ct:ctagbuf plainlen) : MAC.tagB =
-  Buffer.sub ct plainlen MAC.taglen
-
-(* let modifies_table_above_x (#i:id) (t:PRF.state i) *)
-(* 			   (x:PRF.domain i) (h0:mem) (h1 : mem{prf i}) = *)
-(*   let r = PRF.itable i t in *)
-(*   let contents0 = HS.sel h0 r in *)
-(*   let contents1 = HS.sel h1 r in *)
-(*   Seq.length contents0 <= Seq.length contents1 /\ *)
-(*   Seq.equal (Seq.slice contents1 0 (Seq.length contents0)) contents0 /\ *)
-(*   all_above x (Seq.slice contents1 (Seq.length contents0) (Seq.length contents1)) *)
-  
-let enxor_h0_h1
-  (#i:id)
-  (#rw:rw)
-  (#aadlen:aadlen_32)
-  (#plainlen:txtlen_32{plainlen <> 0ul /\ safelen i (v plainlen) (otp_offset i)})
-  (aead_st:aead_state i rw)
-  (nonce:Cipher.iv (alg i))
-  (aad:lbuffer (v aadlen))
-  (plain:plainBuffer i (v plainlen))
-  (cipher_tagged:ctagbuf plainlen)
-  (h0 h1:mem) =
-  let dom_0 = {iv=nonce; ctr=PRF.ctr_0 i} in
-  let cipher = cbuf cipher_tagged in
-  let rgns = Set.as_set [aead_st.prf.rgn; Buffer.frameOf cipher] in
-  HS.(is_stack_region h0.tip) /\
-  HS.(is_stack_region h1.tip) /\  
-  enxor_pre aead_st nonce aad plain cipher h0                 /\
-  enc_dec_liveness_and_separation aead_st aad plain cipher_tagged h1 /\
-  (safeMac i ==>  (
-     let prf = itable i aead_st.prf in
-     let table_0 = HS.sel h0 prf in
-     let table_1 = HS.sel h1 prf in
-     HS.modifies rgns h0 h1                                                            /\
-     HS.modifies_ref aead_st.prf.rgn (TSet.singleton (Heap.Ref (HS.as_ref prf))) h0 h1 /\
-     table_differs_only_above_x (PRF.incr i dom_0) table_0 table_1 /\
-     (safeId i ==> 
-      Seq.equal table_1 (Seq.append table_0
-		                  (counterblocks i aead_st.prf.mac_rgn 
-						 (PRF.incr i dom_0)
-				                 (v plainlen) 0 (v plainlen)
-					         (Plain.sel_plain h1 plainlen plain)
-					         (Buffer.as_seq h1 cipher))))))
-
-val frame_aead_entries_enxor
-  (#i:id)
-  (#rw:rw)
-  (#aadlen:aadlen_32)
-  (#plainlen:nz_ok_len_32 i)
-  (aead_st:aead_state i rw{safeMac i})
-  (nonce:Cipher.iv (alg i))
-  (aad:lbuffer (v aadlen))
-  (plain:plainBuffer i (v plainlen))
-  (ct:ctagbuf plainlen)
-  (h0 h1:mem) : Lemma
-  (requires (enxor_h0_h1 aead_st nonce aad plain ct h0 h1))
-  (ensures  (HS.sel #(aead_entries i) h0 (st_ilog aead_st) ==              
-             HS.sel #(aead_entries i) h1 (st_ilog aead_st)))
-#reset-options "--z3rlimit 50 --initial_fuel 0 --max_fuel 0 --initial_ifuel 0 --max_ifuel 0"
-let frame_aead_entries_enxor #i #rw #aadlen #plainlan aead_st nonce aad plain ct h0 h1 = ()
-
-(*
- * AR: this is also of the above category.
- *)
-val frame_mac_region_enxor
-  (#i:id)
-  (#rw:rw)
-  (#aadlen:aadlen_32)
-  (#plainlen:nz_ok_len_32 i)
-  (aead_st:aead_state i rw{safeMac i})
-  (nonce:Cipher.iv (alg i))
-  (aad:lbuffer (v aadlen))
-  (plain:plainBuffer i (v plainlen))
-  (ct:ctagbuf plainlen)
-  (h0 h1:mem) : Lemma
-  (requires (enxor_h0_h1 aead_st nonce aad plain ct h0 h1))
-  (ensures  (HS.modifies_ref aead_st.prf.mac_rgn TSet.empty h0 h1))
-let frame_mac_region_enxor #i #rw #aadlen #plainlen aead_st nonce aad plain ct h0 h1 = ()
-
-val frame_unused_mac_exists_enxor
-  (#i:id)
-  (#rw:rw)
-  (#aadlen:aadlen_32)
-  (#plainlen:nz_ok_len_32 i)
-  (aead_st:aead_state i rw)
-  (nonce:Cipher.iv (alg i))
-  (aad:lbuffer (v aadlen))
-  (plain:plainBuffer i (v plainlen))
-  (ct:ctagbuf plainlen)
-  (h0 h1:mem) : Lemma
-  (requires (enxor_h0_h1 aead_st nonce aad plain ct h0 h1))
-  (ensures  (safeMac i ==>
-             (let table = HS.sel h1 (itable i aead_st.prf) in
-	      let dom_0 = {iv=nonce; ctr=PRF.ctr_0 i} in
-	      unused_mac_exists table dom_0 h1)))
-#reset-options "--z3rlimit 100 --initial_fuel 0 --max_fuel 0 --initial_ifuel 0 --max_ifuel 0"
-let frame_unused_mac_exists_enxor #i #rw #aadlen #plainlen aead_st nonce aad plain ct h0 h1 =
-  let cipher = cbuf ct in
-  if safeMac i then begin
-    let table_0 = HS.sel h0 (itable i aead_st.prf) in
-    let table_1 = HS.sel h1 (itable i aead_st.prf) in
-    let dom_0 = {iv=nonce; ctr=PRF.ctr_0 i} in
-    frame_mac_region_enxor aead_st nonce aad plain ct h0 h1;
-    frame_unused_mac_exists_h table_0 dom_0 h0 h1;
-    let suffix = Seq.slice table_1 (Seq.length table_0) (Seq.length table_1) in
-    assert (Seq.equal table_1 (Seq.append table_0 suffix));
-    find_mac_all_above_1 suffix nonce;
-    frame_unused_mac_exists_append table_0 dom_0 suffix h1
-  end
-
-let fresh_nonces_are_unused_except (#i:id) (#mac_rgn:region) (nonce:Cipher.iv (alg i))
-				   (prf_table:prf_table mac_rgn i) (aead_entries:aead_entries i) 
-				   (h:mem{safeMac i}) = 
-   forall (nonce':Cipher.iv (alg i)). (fresh_nonce nonce' aead_entries /\ nonce' <> nonce) ==>
-      unused_aead_iv_for_prf prf_table nonce' h
-
-let enxor_and_maybe_mac
-  (#i:id)
-  (#rw:rw)
-  (#aadlen:aadlen_32)
-  (#plainlen:txtlen_32{plainlen <> 0ul /\ safelen i (v plainlen) (otp_offset i)})
-  (maybe_mac:bool)
-  (aead_st:aead_state i rw)
-  (nonce:Cipher.iv (alg i))
-  (aad:lbuffer (v aadlen))
-  (plain:plainBuffer i (v plainlen))
-  (ct:ctagbuf plainlen)
-  (h1:mem) =
-  let cipher = cbuf ct in
-  let tag = ctag ct in 
-  HS.(is_stack_region h1.tip) /\
-  enc_dec_liveness_and_separation aead_st aad plain ct h1 /\
-  (safeMac i ==>
-   (let aead_entries_1 = HS.sel h1 (st_ilog aead_st) in
-    let table_1 = HS.sel h1 (itable i aead_st.prf) in
-    let dom_0 = {iv=nonce; ctr=PRF.ctr_0 i} in
-    fresh_nonce_st nonce aead_st h1 /\
-    fresh_nonces_are_unused_except nonce table_1 aead_entries_1 h1 /\
-    aead_entries_are_refined table_1 aead_entries_1 h1 /\
-    (if maybe_mac 
-     then mac_is_set table_1 nonce (Buffer.as_seq h1 aad) (v plainlen) (Buffer.as_seq h1 cipher) (Buffer.as_seq h1 tag) h1
-     else unused_mac_exists table_1 dom_0 h1) /\
-    (safeId i ==> prf_contains_all_otp_blocks (PRF.incr i dom_0) 0
-	                        (Plain.sel_plain h1 plainlen plain)
-	                        (Buffer.as_seq h1 cipher) table_1)))
-
-val intro_fresh_nonces_are_unused_except 
-  (#i:id)
-  (#rw:rw)
-  (#aadlen:aadlen_32)
-  (#plainlen:nz_ok_len_32 i)
-  (aead_st:aead_state i rw)
-  (nonce:Cipher.iv (alg i))
-  (aad:lbuffer (v aadlen))
-  (plain:plainBuffer i (v plainlen))
-  (ct:ctagbuf plainlen)
-  (h0 h1:mem) 
-  : Lemma
-    (requires (enxor_h0_h1 aead_st nonce aad plain ct h0 h1))
-    (ensures (safeMac i ==>  (
-	      let entries_1   = HS.sel #(aead_entries i) h1 (st_ilog aead_st) in
-	      let table_1     = HS.sel h1 (itable i aead_st.prf) in
-	      fresh_nonces_are_unused_except nonce table_1 entries_1 h1)))
-#reset-options "--z3rlimit 200 --initial_fuel 0 --max_fuel 0 --initial_ifuel 0 --max_ifuel 0"
-let intro_fresh_nonces_are_unused_except 
-  (#i:id)
-  (#rw:rw)
-  (#aadlen:aadlen_32)
-  (#plainlen:nz_ok_len_32 i)
-  (aead_st:aead_state i rw)
-  (nonce:Cipher.iv (alg i))
-  (aad:lbuffer (v aadlen))
-  (plain:plainBuffer i (v plainlen))
-  (ct:ctagbuf plainlen)
-  (h0 h1:mem) =
-  if safeMac i then begin
-      let h1 : (h:mem{safeMac i}) = h1 in
-      let entries_0   = HS.sel #(aead_entries i) h0 (st_ilog aead_st) in
-      let entries_1   = HS.sel #(aead_entries i) h1 (st_ilog aead_st) in
-      let table_0     = HS.sel h0 (itable i aead_st.prf) in
-      let table_1     = HS.sel h1 (itable i aead_st.prf) in
-      let suffix = Seq.slice table_1 (Seq.length table_0) (Seq.length table_1) in
-      let x_1 = {iv = nonce; ctr=otp_offset i} in
-      assert (Seq.equal table_1 (Seq.append table_0 suffix));
-      assert (all_above x_1 suffix);
-      assert (entries_0 == entries_1);
-      assert (fresh_nonce_st nonce aead_st h1);
-      assert (fresh_nonces_are_unused table_0 entries_0 h0);
-      let aux (nonce':Cipher.iv (alg i)) 
-	: Lemma
-	  (requires (fresh_nonce nonce' entries_1 /\ nonce' <> nonce))
-	  (ensures (unused_aead_iv_for_prf table_1 nonce' h1)) = 
-	  assert (unused_aead_iv_for_prf table_0 nonce' h1);
-	  let aux' (y:PRF.domain i{y.iv=nonce'}) 
-	    : Lemma (PRF.find suffix y == None) 
-	    = find_other_iv_all_above suffix x_1 y 
-	  in
-	  FStar.Classical.forall_intro aux';
-	  frame_unused_aead_iv_for_prf_append table_0 suffix h1 nonce' 
-      in	  
-      FStar.Classical.(forall_intro (move_requires aux))
-  end
-
-val lemma_propagate_inv_enxor
-  (#i:id)
-  (#rw:rw)
-  (#aadlen:aadlen_32)
-  (#plainlen:nz_ok_len_32 i)
-  (aead_st:aead_state i rw)
-  (nonce:Cipher.iv (alg i))
-  (aad:lbuffer (v aadlen))
-  (plain:plainBuffer i (v plainlen))
-  (ct:ctagbuf plainlen)
-  (h0 h1:mem) : Lemma
-  (requires (enxor_h0_h1 aead_st nonce aad plain ct h0 h1))
-  (ensures  (enxor_and_maybe_mac false aead_st nonce aad plain ct h1))
-let lemma_propagate_inv_enxor #i #rw #aadlen #plainlen aead_st nonce aad plain ct h0 h1 =
-  let open FStar.Classical in
-  let cipher = cbuf ct in
-  if safeMac i then begin
-    let dom_0 = {iv=nonce; ctr=PRF.ctr_0 i} in
-    let entries_0   = HS.sel #(aead_entries i) h0 (st_ilog aead_st) in
-    let entries_1   = HS.sel #(aead_entries i) h1 (st_ilog aead_st) in
-    let table_0     = HS.sel h0 (itable i aead_st.prf) in
-    let table_1     = HS.sel h1 (itable i aead_st.prf) in
-    assert (entries_0 == entries_1);
-    assert (fresh_nonce_st nonce aead_st h1);
-    intro_fresh_nonces_are_unused_except aead_st nonce aad plain ct h0 h1;
-    frame_aead_entries_enxor aead_st nonce aad plain ct h0 h1;
-    frame_mac_region_enxor   aead_st nonce aad plain ct h0 h1;
-    frame_unused_mac_exists_enxor aead_st nonce aad plain ct h0 h1;
-    frame_refines_entries_h i aead_st.prf.mac_rgn table_0 entries_1 h0 h1;
-    if safeId i then begin
-      let otp_blocks = counterblocks i aead_st.prf.mac_rgn (PRF.incr i dom_0)
-    		                   (v plainlen) 0 (v plainlen)
-    			           (Plain.sel_plain h1 plainlen plain)
-    			           (Buffer.as_seq h1 cipher) in
-
-      frame_refines_entries_prf_append table_0 entries_1 h1 otp_blocks;
-      frame_prf_contains_all_otp_blocks_prefix 
-	  (PRF.incr i dom_0) 
-	  (Plain.sel_plain h1 plainlen plain)
-    	  (Buffer.as_seq h1 cipher) 
-	  table_0
-     end					     
-  end
-
-val lemma_propagate_inv_accumulate
-  (#i:id)
-  (#rw:rw)
-  (#aadlen:aadlen_32)
-  (#plainlen:txtlen_32{plainlen <> 0ul /\ safelen i (v plainlen) (otp_offset i)})
-  (maybe_mac:bool)
-  (aead_st:aead_state i rw)
-  (nonce:Cipher.iv (alg i))
-  (aad:lbuffer (v aadlen))
-  (plain:plainBuffer i (v plainlen))
-  (ct:ctagbuf plainlen)
-  (h0 h1:mem) : Lemma
-  (requires (enxor_and_maybe_mac maybe_mac aead_st nonce aad plain ct h0 /\
-	     Buffer.modifies_0 h0 h1))
-  (ensures  (enxor_and_maybe_mac maybe_mac aead_st nonce aad plain ct h1))
-let lemma_propagate_inv_accumulate #i #rw #aadlen #plainlen maybe_mac aead_st nonce aad plain ct h0 h1 =
-  let open FStar.Classical in
-  Buffer.lemma_reveal_modifies_0 h0 h1;
-  let cipher = cbuf ct in
-  let tag = ctag ct in
-  assert (Plain.sel_plain h0 plainlen plain == Plain.sel_plain h1 plainlen plain);
-  let ad_0      = Buffer.as_seq h0 aad in
-  let ad_1      = Buffer.as_seq h1 aad in
-  let c0 = Buffer.as_seq h0 cipher in
-  let c1 = Buffer.as_seq h1 cipher in
-  let t0 = Buffer.as_seq h0 tag in
-  let t1 = Buffer.as_seq h0 tag in  
-  assert (c0 == c1);
-  assert (ad_0 == ad_1);
-  assert (t0 == t1);
-  if safeMac i then begin
-    let dom_0 = {iv=nonce; ctr=PRF.ctr_0 i} in
-    let entries_0 = HS.sel #(aead_entries i) h0 (st_ilog aead_st) in
-    let table_0   = HS.sel h0 (itable i aead_st.prf) in
-
-    let entries_1 = HS.sel #(aead_entries i) h1 (st_ilog aead_st) in
-    let table_1   = HS.sel h1 (itable i aead_st.prf) in    
-
-    assert (table_0 == table_1);
-    assert (entries_0 == entries_1);
-    frame_refines_entries_h i aead_st.prf.mac_rgn table_0 entries_0 h0 h1;
-
-    if maybe_mac 
-    then frame_mac_is_set_h table_0 nonce ad_0 (v plainlen) c0 t0 h0 h1
-    else frame_unused_mac_exists_h table_0 dom_0 h0 h1
-  end
-
-val lemma_mac_log_framing
-  (#i:id)
-  (nonce_1:Cipher.iv (alg i){safeMac i})
-  (mac_st_1:CMA.state (i, nonce_1))
-  (h0 h1:mem)
-  (nonce_2:Cipher.iv (alg i))
-  (mac_st_2:CMA.state (i, nonce_2){CMA.(mac_st_2.region) = CMA.(mac_st_1.region)}) : Lemma
-  (requires (nonce_1 <> nonce_2                                       /\
-             m_contains (CMA.(ilog mac_st_2.log)) h0                /\
-	     HS.(h1.h `Map.contains` CMA.(mac_st_2.region))          /\
-             HS.modifies_ref (CMA.(mac_st_1.region)) !{HS.as_ref (as_hsref (CMA.(ilog mac_st_1.log)))} h0 h1))
-  (ensures  (m_sel h0 (CMA.(ilog mac_st_2.log)) = m_sel h1 (CMA.(ilog mac_st_2.log))))
-#set-options "--initial_ifuel 1 --max_ifuel 1"
-let lemma_mac_log_framing #i nonce_1 mac_st_1 h0 h1 nonce_2 mac_st_2 = ()
-#set-options "--initial_ifuel 0 --max_ifuel 0"
-
-let lemma_fresh_nonce_implies_all_entries_nonces_are_different
-  (#i:id)
-  (aead_entries:aead_entries i)
-  (nonce:Cipher.iv (alg i)) : Lemma
-  (requires (fresh_nonce nonce aead_entries))
-  (ensures  (forall (e:aead_entry i).{:pattern (aead_entries `SeqProperties.contains` e)}
-	        aead_entries `SeqProperties.contains` e ==> e.nonce <> nonce))
-  = let open FStar.Classical in
-    move_requires (SeqProperties.find_l_none_no_index aead_entries) (is_aead_entry_nonce nonce);
-    forall_intro (SeqProperties.contains_elim aead_entries)
-
-let mac_wrapper_h0_h1
-  (#i:id)
-  (#rw:rw)
-  (#aadlen:aadlen_32)
-  (#plainlen:nz_ok_len_32 i)
-  (aead_st:aead_state i rw)
-  (nonce:Cipher.iv (alg i))
-  (aad:lbuffer (v aadlen))
-  (plain:plainBuffer i (v plainlen))
-  (ct:ctagbuf plainlen)
-  (mac_st:CMA.state (i, nonce))
-  (h0 h1:mem) =
-  let cipher = cbuf ct in
-  let tag = ctag ct in
-  HS.(is_stack_region h0.tip) /\
-  HS.(is_stack_region h1.tip) /\  
-  enxor_and_maybe_mac false aead_st nonce aad plain ct h0 /\
-  enc_dec_liveness_and_separation aead_st aad plain ct h1 /\
-  CMA.(mac_st.region = aead_st.prf.mac_rgn) /\
-  (safeMac i ==>  (
-    let prf_table_1 = HS.sel h1 (itable i aead_st.prf) in
-    HS.modifies (Set.as_set [h0.tip; aead_st.prf.mac_rgn; Buffer.frameOf ct]) h0 h1 /\
-    HS.modifies_ref aead_st.prf.mac_rgn !{HS.as_ref (as_hsref (CMA.(ilog mac_st.log)))} h0 h1  /\
-    Buffer.modifies_buf_1 (Buffer.frameOf ct) tag h0 h1 /\
-    mac_is_set prf_table_1 nonce (Buffer.as_seq h1 aad) (v plainlen) (Buffer.as_seq h1 cipher) (Buffer.as_seq h1 tag) h1))
-
-val frame_aead_entries_are_refined_mac_wrapper
-  (#i:id)
-  (#rw:rw)
-  (#aadlen:aadlen_32)
-  (#plainlen:nz_ok_len_32 i)
-  (aead_st:aead_state i rw)
-  (nonce:Cipher.iv (alg i))
-  (aad:lbuffer (v aadlen))
-  (plain:plainBuffer i (v plainlen))
-  (cipher_tagged:lbuffer (v plainlen + v MAC.taglen))
-  (mac_st:CMA.state (i, nonce))
-  (h0 h1:mem) : Lemma
-  (requires (mac_wrapper_h0_h1 aead_st nonce aad plain cipher_tagged mac_st h0 h1))
-  (ensures  (safeId i ==>
-             (let entries_0 = HS.sel #(aead_entries i) h0 (st_ilog aead_st) in
-	      let table_0 = HS.sel h0 (itable i aead_st.prf) in
-	      let entries_1 = HS.sel h1 (st_ilog aead_st) in
-	      let table_1 = HS.sel h1 (itable i aead_st.prf) in
-	      entries_0 == entries_1 /\
-	      table_0 == table_1 /\
-	      aead_entries_are_refined table_0 entries_0 h1)))
-#set-options "--z3rlimit 200"
-let frame_aead_entries_are_refined_mac_wrapper #i #rw #aadlen #plainlen aead_st nonce aad plain cipher_tagged mac_st h0 h1 =
-  let open FStar.SeqProperties in
-  if safeId i then begin
-    let entries_0 = HS.sel h0 (st_ilog aead_st) in
-    let table_0 = HS.sel h0 (itable i aead_st.prf) in
-    let entries_1 = HS.sel h1 (st_ilog aead_st) in
-    let table_1 = HS.sel h1 (itable i aead_st.prf) in
-    assert (entries_0 == entries_1);
-    assert (table_0 == table_1);    
-    assert (aead_entries_are_refined table_0 entries_0 h0);
-    let h1: (h:HS.mem{safeId i}) = h1 in
-    let aux (e:aead_entry i) : Lemma
-    	(requires (entries_1 `contains` e))
-	(ensures (refines_one_entry table_1 e h1)) =  //TODO: This proof is rather indirect; could be spelled out more
-	lemma_fresh_nonce_implies_all_entries_nonces_are_different entries_1 nonce in
-    FStar.Classical.(forall_intro (move_requires aux))
-  end
-
-val frame_unused_aead_id_for_prf_mac_wrapper
-  (#i:id)
-  (#rw:rw)
-  (#aadlen:aadlen_32)
-  (#plainlen:nz_ok_len_32 i)
-  (aead_st:aead_state i rw{safeMac i})
-  (nonce:Cipher.iv (alg i))
-  (aad:lbuffer (v aadlen))
-  (plain:plainBuffer i (v plainlen))
-  (ct:ctagbuf plainlen)
-  (mac_st:CMA.state (i, nonce))
-  (h0 h1:mem)
-  (nonce':Cipher.iv (alg i)) : Lemma
-  (requires (let table_0 = HS.sel h0 (itable i aead_st.prf) in
-             mac_wrapper_h0_h1 aead_st nonce aad plain ct mac_st h0 h1 /\
-             unused_aead_iv_for_prf table_0 nonce' h0 /\
-	     nonce <> nonce'))
-  (ensures  (let table_0 = HS.sel h0 (itable i aead_st.prf) in
-             unused_aead_iv_for_prf table_0 nonce' h1))
-#reset-options "--z3rlimit 100 --initial_fuel 0 --max_fuel 0 --initial_ifuel 0 --max_ifuel 0"
-let frame_unused_aead_id_for_prf_mac_wrapper #i #rw #aadlen #plainlen aead_st nonce aad plain ct mac_st h0 h1 nonce' =
-   let dom_0 = {iv=nonce'; ctr=PRF.ctr_0 i} in
-   let prf_table = HS.sel h0 (itable i aead_st.prf) in
-   assert (none_above (PRF.incr i dom_0) prf_table)
-   (match PRF.find_mac prf_table dom_0 with
-    | None           -> ()
-    | Some mac_range -> 
-      assert (CMA.mac_is_unset (i, nonce') aead_st.prf.mac_rgn mac_range h0);
-      MAC.frame_norm h0 h1 CMA.(mac_range.r);
-      lemma_mac_log_framing nonce mac_st h0 h1 nonce' mac_range)
-
-#reset-options "--z3rlimit 100 --initial_fuel 0 --max_fuel 0 --initial_ifuel 0 --max_ifuel 0"      
-val frame_unused_aead_id_for_prf_mac_wrapper_forall
-  (#i:id)
-  (#rw:rw)
-  (#aadlen:aadlen_32)
-  (#plainlen:nz_ok_len_32 i)
-  (aead_st:aead_state i rw{safeMac i})
-  (nonce:Cipher.iv (alg i))
-  (aad:lbuffer (v aadlen))
-  (plain:plainBuffer i (v plainlen))
-  (cipher_tagged:ctagbuf plainlen)
-  (mac_st:CMA.state (i, nonce))
-  (h0 h1:mem) : Lemma
-  (requires (mac_wrapper_h0_h1 aead_st nonce aad plain cipher_tagged mac_st h0 h1))
-  (ensures  (let table_0 = HS.sel h0 (itable i aead_st.prf) in
-             forall (nonce':Cipher.iv (alg i)). (nonce' <> nonce /\ unused_aead_iv_for_prf table_0 nonce' h0) ==>
-	                                   unused_aead_iv_for_prf table_0 nonce' h1))
-let frame_unused_aead_id_for_prf_mac_wrapper_forall #i #rw #aadlen #plainlen aead_st nonce aad plain cipher_tagged mac_st h0 h1 =
-  let open FStar.Classical in
-  forall_intro (move_requires (frame_unused_aead_id_for_prf_mac_wrapper aead_st nonce aad plain cipher_tagged mac_st h0 h1))
-
-val frame_entries_and_table_mac_wrapper
-  (#i:id)
-  (#rw:rw)
-  (#aadlen:aadlen_32) 
-  (#plainlen:nz_ok_len_32 i)
-  (aead_st:aead_state i rw)
-  (nonce:Cipher.iv (alg i))
-  (aad:lbuffer (v aadlen))
-  (plain:plainBuffer i (v plainlen))
-  (cipher_tagged:ctagbuf plainlen)
-  (mac_st:CMA.state (i, nonce))
-  (h0 h1:mem) : Lemma
-  (requires (mac_wrapper_h0_h1 aead_st nonce aad plain cipher_tagged mac_st h0 h1))
-  (ensures  (safeMac i ==>
-             (let entries_0 = HS.sel #(aead_entries i) h0 (st_ilog aead_st) in
-              let entries_1 = HS.sel #(aead_entries i) h1 (st_ilog aead_st) in
-	      let table_0 = HS.sel h0 (itable i aead_st.prf) in
-	      let table_1 = HS.sel h1 (itable i aead_st.prf) in
-	      entries_0 == entries_1 /\ table_0 == table_1)))
-let frame_entries_and_table_mac_wrapper #i #rw #aadlen #plainlen aead_st nonce aad plain cipher_tagged mac_st h0 h1 = 
-  frame_aead_entries_are_refined_mac_wrapper aead_st nonce aad plain cipher_tagged mac_st h0 h1
 
 #reset-options "--z3rlimit 200 --initial_fuel 0 --max_fuel 0 --initial_ifuel 0 --max_ifuel 0"      
-let frame_plain_and_cipher
-  (#i:id)
-  (#rw:rw)
-  (#aadlen:aadlen_32)
-  (#plainlen:nz_ok_len_32 i)
-  (aead_st:aead_state i rw)
-  (nonce:Cipher.iv (alg i))
-  (aad:lbuffer (v aadlen))
-  (plain:plainBuffer i (v plainlen))
-  (ct:ctagbuf plainlen)
-  (mac_st:CMA.state (i, nonce))
-  (h0 h1:mem) : Lemma
-  (requires (mac_wrapper_h0_h1 aead_st nonce aad plain ct mac_st h0 h1))
-  (ensures (mac_wrapper_h0_h1 aead_st nonce aad plain ct mac_st h0 h1 /\
-	   (safeMac i ==> 
-	       Plain.sel_plain h0 plainlen plain == Plain.sel_plain h1 plainlen plain /\
-	       Buffer.as_seq h0 (cbuf ct) == Buffer.as_seq h1 (cbuf ct)))) = ()
-	       
-val lemma_propagate_inv_mac_wrapper
-  (#i:id)
-  (#rw:rw)
-  (#aadlen:aadlen_32)
-  (#plainlen:nz_ok_len_32 i)
-  (aead_st:aead_state i rw)
-  (nonce:Cipher.iv (alg i))
-  (aad:lbuffer (v aadlen))
-  (plain:plainBuffer i (v plainlen))
-  (ct:ctagbuf plainlen)
-  (mac_st:CMA.state (i, nonce))
-  (h0 h1:mem) : Lemma
-  (requires (mac_wrapper_h0_h1 aead_st nonce aad plain ct mac_st h0 h1))
-  (ensures  (enxor_and_maybe_mac true aead_st nonce aad plain ct h1))
-let lemma_propagate_inv_mac_wrapper #i #rw #aadlen #plainlen aead_st nonce aad plain cipher_tagged mac_st h0 h1 =
-  let open FStar.Classical in 
-  if safeMac i 
-  then begin 
-    frame_plain_and_cipher                          aead_st nonce aad plain cipher_tagged mac_st h0 h1;
-    frame_entries_and_table_mac_wrapper             aead_st nonce aad plain cipher_tagged mac_st h0 h1;
-    frame_aead_entries_are_refined_mac_wrapper      aead_st nonce aad plain cipher_tagged mac_st h0 h1;
-    frame_unused_aead_id_for_prf_mac_wrapper_forall aead_st nonce aad plain cipher_tagged mac_st h0 h1
-  end
-
 let safeMac_ideal_writes 
   (#i:id)
   (#rw:rw)
@@ -973,7 +426,7 @@ let safeMac_ideal_writes
 		      (AEADEntry nonce 
 				 (Buffer.as_seq h0 aad) 
 				 (v plainlen) 
-				 (Plain.sel_plain h0 plainlen plain) 
+				 (sel_plain h0 plainlen plain) 
 				 (Buffer.as_seq h0 ct))
    else h0 == h1)
 
@@ -995,7 +448,7 @@ val frame_ideal_writes
 	       let table_0 = HS.sel h0 (itable i aead_st.prf) in
 	       let table_1 = HS.sel h1 (itable i aead_st.prf) in
 	       table_0 == table_1 /\
-	       Plain.sel_plain h0 plainlen plain == Plain.sel_plain h1 plainlen plain /\
+	       sel_plain h0 plainlen plain == sel_plain h1 plainlen plain /\
 	       Buffer.as_seq h0 ct == Buffer.as_seq h1 ct                             /\
 	       Buffer.as_seq h0 aad == Buffer.as_seq h1 aad                           /\
 	       HS.modifies_ref aead_st.prf.mac_rgn TSet.empty h0 h1))))
@@ -1026,7 +479,7 @@ let fresh_nonces_are_unused_after_ideal #i #rw #aadlen #plainlen aead_st nonce a
     let entries_0 = HS.sel h0 (st_ilog aead_st) in
     let c = Buffer.as_seq h0 ct in
     let ad = Buffer.as_seq h0 aad in
-    let p = Plain.sel_plain h0 plainlen plain in
+    let p = sel_plain h0 plainlen plain in
     let entry = AEADEntry nonce ad (v plainlen) p c in
     let entries_1 = HS.sel h1 (st_ilog aead_st) in 
     let prf_table = HS.sel h0 (PRF.itable i aead_st.prf) in
@@ -1074,7 +527,7 @@ let reestablish_inv #i #rw #aadlen #plainlen aead_st nonce aad plain ct h0 h1 =
     let t = Buffer.as_seq h0 tag in
     let c = Buffer.as_seq h0 cipher in
     let ad = Buffer.as_seq h0 aad in
-    let p = Plain.sel_plain h0 plainlen plain in
+    let p = sel_plain h0 plainlen plain in
     let entries_0 = HS.sel h0 (st_ilog aead_st) in
     let entry = AEADEntry nonce ad (v plainlen) p (Buffer.as_seq h0 ct) in    
     let entries_1 = SeqProperties.snoc entries_0 entry in
